Updated examples.

tests/List.bpl
@@ -13,7 +13,6 @@ var R: CType;
 var C#init: CType;
 var St: [Actor]State;
 
-
 const unique this#: Actor;
 
 type List a = [int]a;
@@ -27,13 +26,15 @@ var AT#intlst: List int;
 procedure ListTest#anon$0#0()
   modifies C, R, M, St;
 {
+  var Chip_map_table: List (int);
   var X: List (int);
   var IV#in#i: int;
-  var ActionVar#o: int;
-  assume (X[0] == 10) && (X[1] == 11) && (X[2] == 12);
+  assume X == AT#intlst[0 := 10][1 := 11][2 := 12];
+  assume Chip_map_table == AT#intlst[0 := 1951056795][1 := 1152137655][2 := 1254333300][3 := 2889463620][4 := 3281744970][5 := 968311980][6 := 2608089795][7 := 3074731065][8 := 3739248945][9 := 3993408285][10 := 3764990430][11 := 110304750][12 := 1764876000][13 := 2468212230][14 := 836690025][15 := 502138515];
   assume (0 <= IV#in#i) && (IV#in#i < 3);
-  ActionVar#o := X[IV#in#i];
-  assert {:msg "  3.13: Action might not preserve invariant"} (X[0] == 10) && (X[1] == 11) && (X[2] == 12);
+  assume true;
+  assert {:msg "  11.13: Action might not preserve invariant"} X == AT#intlst[0 := 10][1 := 11][2 := 12];
+  assert {:msg "  12.13: Action might not preserve invariant"} Chip_map_table == AT#intlst[0 := 1951056795][1 := 1152137655][2 := 1254333300][3 := 2889463620][4 := 3281744970][5 := 968311980][6 := 2608089795][7 := 3074731065][8 := 3739248945][9 := 3993408285][10 := 3764990430][11 := 110304750][12 := 1764876000][13 := 2468212230][14 := 836690025][15 := 502138515];
 }
 const unique Net#l: Actor;
 const unique Net#a: Chan (int);
@@ -54,20 +55,21 @@ procedure Net#anon$1#entry#1()
   assert {:msg "  Channel invariant might not hold on action entry (generated #3)"} 0 <= R[Net#b];
   assert {:msg "  Channel invariant might not hold on action entry (generated #4)"} 0 <= C[Net#b];
   assert {:msg "  Channel invariant might not hold on action entry (generated #5)"} R[Net#b] == 0;
-  assert {:msg "  22.3: Channel invariant might not hold on action entry"} (0 <= M[Net#a][0]) && (M[Net#a][0] < 3);
-  assert {:msg "  23.3: Channel invariant might not hold on action entry"} R[Net#a] == (R[Net#b] + C[Net#b]);
-  assert {:msg "  24.3: Channel invariant might not hold on action entry"} (forall i: int :: 
+  assert {:msg "  Channel invariant might not hold on action entry (generated #6)"} (0 <= M[Net#a][0]) && (M[Net#a][0] < 3);
+  assert {:msg "  30.3: Channel invariant might not hold on action entry"} (0 <= M[Net#a][0]) && (M[Net#a][0] < 3);
+  assert {:msg "  31.3: Channel invariant might not hold on action entry"} R[Net#a] == (R[Net#b] + C[Net#b]);
+  assert {:msg "  32.3: Channel invariant might not hold on action entry"} (forall i: int :: 
     (0 <= i) && (i < (R[Net#b] + C[Net#b])) ==> (10 <= M[Net#b][i]) && (M[Net#b][i] <= 12)
   );
-  assert {:msg "  25.3: Channel invariant might not hold on action entry"} (forall i: int :: 
+  assert {:msg "  33.3: Channel invariant might not hold on action entry"} (forall i: int :: 
     (0 <= i) && (i < (R[Net#b] + C[Net#b])) ==> ((M[Net#a][i] == 0) ==> (M[Net#b][i] == 10))
   );
 }
 procedure Net#anon$1#ListTest#anon$0#2()
   modifies C, R, M, St;
 {
+  var ActorVar#Chip_map_table: List (int);
   var ActorVar#X: List (int);
-  var ActionVar#o: int;
   var St#next: State;
   var in#i: int;
   assume C#init[Net#a] == 1;
@@ -79,6 +81,7 @@ procedure Net#anon$1#ListTest#anon$0#2()
   assume 0 <= C[Net#b];
   assume R[Net#b] == 0;
   assume (0 <= M[Net#a][0]) && (M[Net#a][0] < 3);
+  assume (0 <= M[Net#a][0]) && (M[Net#a][0] < 3);
   assume R[Net#a] == (R[Net#b] + C[Net#b]);
   assume (forall i: int :: 
     (0 <= i) && (i < (R[Net#b] + C[Net#b])) ==> (10 <= M[Net#b][i]) && (M[Net#b][i] <= 12)
@@ -89,24 +92,26 @@ procedure Net#anon$1#ListTest#anon$0#2()
   assume (0 <= M[Net#a][R[Net#a] - 0]) && (M[Net#a][R[Net#a] - 0] < 3);
   assume true;
   assume (1 <= C[Net#a]) && (0 <= M[Net#a][R[Net#a] - 0]) && (M[Net#a][R[Net#a] - 0] < 3);
-  assume (ActorVar#X[0] == 10) && (ActorVar#X[1] == 11) && (ActorVar#X[2] == 12);
+  assume ActorVar#X == AT#intlst[0 := 10][1 := 11][2 := 12];
+  assume ActorVar#Chip_map_table == AT#intlst[0 := 1951056795][1 := 1152137655][2 := 1254333300][3 := 2889463620][4 := 3281744970][5 := 968311980][6 := 2608089795][7 := 3074731065][8 := 3739248945][9 := 3993408285][10 := 3764990430][11 := 110304750][12 := 1764876000][13 := 2468212230][14 := 836690025][15 := 502138515];
   in#i := M[Net#a][R[Net#a]];
   R[Net#a] := R[Net#a] + 1;
   C[Net#a] := C[Net#a] - 1;
   M[Net#b][R[Net#b] + C[Net#b]] := ActorVar#X[in#i];
   C[Net#b] := C[Net#b] + 1;
-  assert {:msg "  Sub-actor action at 7.3 might not preserve the channel invariant (generated #6)"} 0 <= R[Net#a];
-  assert {:msg "  Sub-actor action at 7.3 might not preserve the channel invariant (generated #7)"} 0 <= C[Net#a];
-  assert {:msg "  Sub-actor action at 7.3 might not preserve the channel invariant (generated #8)"} (R[Net#a] + C[Net#a]) == C#init[Net#a];
-  assert {:msg "  Sub-actor action at 7.3 might not preserve the channel invariant (generated #9)"} 0 <= R[Net#b];
-  assert {:msg "  Sub-actor action at 7.3 might not preserve the channel invariant (generated #10)"} 0 <= C[Net#b];
-  assert {:msg "  Sub-actor action at 7.3 might not preserve the channel invariant (generated #11)"} R[Net#b] == 0;
-  assert {:msg "  22.3: Sub-actor action at 7.3 might not preserve the channel invariant"} (0 <= M[Net#a][0]) && (M[Net#a][0] < 3);
-  assert {:msg "  23.3: Sub-actor action at 7.3 might not preserve the channel invariant"} R[Net#a] == (R[Net#b] + C[Net#b]);
-  assert {:msg "  24.3: Sub-actor action at 7.3 might not preserve the channel invariant"} (forall i: int :: 
+  assert {:msg "  Sub-actor action at 18.3 might not preserve the channel invariant (generated #7)"} 0 <= R[Net#a];
+  assert {:msg "  Sub-actor action at 18.3 might not preserve the channel invariant (generated #8)"} 0 <= C[Net#a];
+  assert {:msg "  Sub-actor action at 18.3 might not preserve the channel invariant (generated #9)"} (R[Net#a] + C[Net#a]) == C#init[Net#a];
+  assert {:msg "  Sub-actor action at 18.3 might not preserve the channel invariant (generated #10)"} 0 <= R[Net#b];
+  assert {:msg "  Sub-actor action at 18.3 might not preserve the channel invariant (generated #11)"} 0 <= C[Net#b];
+  assert {:msg "  Sub-actor action at 18.3 might not preserve the channel invariant (generated #12)"} R[Net#b] == 0;
+  assert {:msg "  Sub-actor action at 18.3 might not preserve the channel invariant (generated #13)"} (0 <= M[Net#a][0]) && (M[Net#a][0] < 3);
+  assert {:msg "  30.3: Sub-actor action at 18.3 might not preserve the channel invariant"} (0 <= M[Net#a][0]) && (M[Net#a][0] < 3);
+  assert {:msg "  31.3: Sub-actor action at 18.3 might not preserve the channel invariant"} R[Net#a] == (R[Net#b] + C[Net#b]);
+  assert {:msg "  32.3: Sub-actor action at 18.3 might not preserve the channel invariant"} (forall i: int :: 
     (0 <= i) && (i < (R[Net#b] + C[Net#b])) ==> (10 <= M[Net#b][i]) && (M[Net#b][i] <= 12)
   );
-  assert {:msg "  25.3: Sub-actor action at 7.3 might not preserve the channel invariant"} (forall i: int :: 
+  assert {:msg "  33.3: Sub-actor action at 18.3 might not preserve the channel invariant"} (forall i: int :: 
     (0 <= i) && (i < (R[Net#b] + C[Net#b])) ==> ((M[Net#a][i] == 0) ==> (M[Net#b][i] == 10))
   );
 }
@@ -123,6 +128,7 @@ procedure Net#anon$1#exit#3()
   assume 0 <= C[Net#b];
   assume R[Net#b] == 0;
   assume (0 <= M[Net#a][0]) && (M[Net#a][0] < 3);
+  assume (0 <= M[Net#a][0]) && (M[Net#a][0] < 3);
   assume R[Net#a] == (R[Net#b] + C[Net#b]);
   assume (forall i: int :: 
     (0 <= i) && (i < (R[Net#b] + C[Net#b])) ==> (10 <= M[Net#b][i]) && (M[Net#b][i] <= 12)
@@ -131,10 +137,10 @@ procedure Net#anon$1#exit#3()
     (0 <= i) && (i < (R[Net#b] + C[Net#b])) ==> ((M[Net#a][i] == 0) ==> (M[Net#b][i] == 10))
   );
   assume !((1 <= C[Net#a]) && (0 <= M[Net#a][R[Net#a] - 0]) && (M[Net#a][R[Net#a] - 0] < 3));
-  assert {:msg "  16.3: The network might leave unread tokens on channel a"} C[Net#a] == 0;
-  assert {:msg "  16.3: The network might not produce the specified number of tokens on output out"} C[Net#b] == 1;
+  assert {:msg "  24.3: The network might leave unread tokens on channel a"} C[Net#a] == 0;
+  assert {:msg "  24.3: The network might not produce the specified number of tokens on output out"} C[Net#b] == 1;
   ActionVar#y := M[Net#b][0];
-  assert {:msg "  19.14: Postcondition might not hold"} (M[Net#a][0] == 0) ==> (ActionVar#y == 10);
+  assert {:msg "  27.14: Postcondition might not hold"} (M[Net#a][0] == 0) ==> (ActionVar#y == 10);
   R[Net#b] := R[Net#b] + C[Net#b];
   C[Net#b] := 0;
 }
