tests/DataDependent.bpl
@@ -82,17 +82,17 @@ procedure Net#anon$3#entry#3()
   assert {:msg "  Channel invariant might not hold on action entry (generated #8)"} 0 <= R[Net#d];
   assert {:msg "  Channel invariant might not hold on action entry (generated #9)"} 0 <= C[Net#d];
   assert {:msg "  Channel invariant might not hold on action entry (generated #10)"} R[Net#d] == 0;
-  assert {:msg "  Channel invariant might not hold on action entry (generated #11)"} R[Net#a] == (R[Net#b] + C[Net#b]);
-  assert {:msg "  Channel invariant might not hold on action entry (generated #12)"} (forall idx$: int :: 
+  assert {:msg "  Channel invariant might not hold on action entry (generated #11)"} (M[Net#a][0] < 0) && (M[Net#a][1] > 0);
+  assert {:msg "  Channel invariant might not hold on action entry (generated #12)"} R[Net#a] == (R[Net#b] + C[Net#b]);
+  assert {:msg "  Channel invariant might not hold on action entry (generated #13)"} (forall idx$: int :: 
     (0 <= idx$) && (idx$ < (R[Net#b] + C[Net#b])) ==> (M[Net#b][idx$] == M[Net#a][idx$])
   );
-  assert {:msg "  20.3: Channel invariant might not hold on action entry"} (M[Net#a][0] < 0) && (M[Net#a][1] > 0);
-  assert {:msg "  21.3: Channel invariant might not hold on action entry"} (R[Net#d] + C[Net#d]) == AT#Div(R[Net#b] + 1, 2);
-  assert {:msg "  22.3: Channel invariant might not hold on action entry"} (R[Net#c] + C[Net#c]) == AT#Div(R[Net#b], 2);
-  assert {:msg "  23.3: Channel invariant might not hold on action entry"} (forall i: int :: 
+  assert {:msg "  20.3: Channel invariant might not hold on action entry"} (R[Net#d] + C[Net#d]) == AT#Div(R[Net#b] + 1, 2);
+  assert {:msg "  21.3: Channel invariant might not hold on action entry"} (R[Net#c] + C[Net#c]) == AT#Div(R[Net#b], 2);
+  assert {:msg "  22.3: Channel invariant might not hold on action entry"} (forall i: int :: 
     (0 <= i) && (i < R[Net#b]) && (AT#Mod(i, 2) == 0) ==> (M[Net#b][i] == M[Net#d][AT#Div(i, 2)])
   );
-  assert {:msg "  24.3: Channel invariant might not hold on action entry"} (forall i: int :: 
+  assert {:msg "  23.3: Channel invariant might not hold on action entry"} (forall i: int :: 
     (0 <= i) && (i < R[Net#b]) && (AT#Mod(i, 2) == 1) ==> (M[Net#b][i] == M[Net#c][AT#Div(i, 2)])
   );
 }
@@ -116,11 +116,11 @@ procedure Net#anon$3#Repeater#anon$0#4()
   assume 0 <= R[Net#d];
   assume 0 <= C[Net#d];
   assume R[Net#d] == 0;
+  assume (M[Net#a][0] < 0) && (M[Net#a][1] > 0);
   assume R[Net#a] == (R[Net#b] + C[Net#b]);
   assume (forall idx$: int :: 
     (0 <= idx$) && (idx$ < (R[Net#b] + C[Net#b])) ==> (M[Net#b][idx$] == M[Net#a][idx$])
   );
-  assume (M[Net#a][0] < 0) && (M[Net#a][1] > 0);
   assume (R[Net#d] + C[Net#d]) == AT#Div(R[Net#b] + 1, 2);
   assume (R[Net#c] + C[Net#c]) == AT#Div(R[Net#b], 2);
   assume (forall i: int :: 
@@ -136,28 +136,28 @@ procedure Net#anon$3#Repeater#anon$0#4()
   C[Net#a] := C[Net#a] - 1;
   M[Net#b][R[Net#b] + C[Net#b]] := in#i;
   C[Net#b] := C[Net#b] + 1;
-  assert {:msg "  Sub-actor action at 3.3 might not preserve the channel invariant (generated #13)"} 0 <= R[Net#a];
-  assert {:msg "  Sub-actor action at 3.3 might not preserve the channel invariant (generated #14)"} 0 <= C[Net#a];
-  assert {:msg "  Sub-actor action at 3.3 might not preserve the channel invariant (generated #15)"} (R[Net#a] + C[Net#a]) == C#init[Net#a];
-  assert {:msg "  Sub-actor action at 3.3 might not preserve the channel invariant (generated #16)"} 0 <= R[Net#b];
-  assert {:msg "  Sub-actor action at 3.3 might not preserve the channel invariant (generated #17)"} 0 <= C[Net#b];
-  assert {:msg "  Sub-actor action at 3.3 might not preserve the channel invariant (generated #18)"} 0 <= R[Net#c];
-  assert {:msg "  Sub-actor action at 3.3 might not preserve the channel invariant (generated #19)"} 0 <= C[Net#c];
-  assert {:msg "  Sub-actor action at 3.3 might not preserve the channel invariant (generated #20)"} R[Net#c] == 0;
-  assert {:msg "  Sub-actor action at 3.3 might not preserve the channel invariant (generated #21)"} 0 <= R[Net#d];
-  assert {:msg "  Sub-actor action at 3.3 might not preserve the channel invariant (generated #22)"} 0 <= C[Net#d];
-  assert {:msg "  Sub-actor action at 3.3 might not preserve the channel invariant (generated #23)"} R[Net#d] == 0;
-  assert {:msg "  Sub-actor action at 3.3 might not preserve the channel invariant (generated #24)"} R[Net#a] == (R[Net#b] + C[Net#b]);
-  assert {:msg "  Sub-actor action at 3.3 might not preserve the channel invariant (generated #25)"} (forall idx$: int :: 
+  assert {:msg "  Sub-actor action at 3.3 might not preserve the channel invariant (generated #14)"} 0 <= R[Net#a];
+  assert {:msg "  Sub-actor action at 3.3 might not preserve the channel invariant (generated #15)"} 0 <= C[Net#a];
+  assert {:msg "  Sub-actor action at 3.3 might not preserve the channel invariant (generated #16)"} (R[Net#a] + C[Net#a]) == C#init[Net#a];
+  assert {:msg "  Sub-actor action at 3.3 might not preserve the channel invariant (generated #17)"} 0 <= R[Net#b];
+  assert {:msg "  Sub-actor action at 3.3 might not preserve the channel invariant (generated #18)"} 0 <= C[Net#b];
+  assert {:msg "  Sub-actor action at 3.3 might not preserve the channel invariant (generated #19)"} 0 <= R[Net#c];
+  assert {:msg "  Sub-actor action at 3.3 might not preserve the channel invariant (generated #20)"} 0 <= C[Net#c];
+  assert {:msg "  Sub-actor action at 3.3 might not preserve the channel invariant (generated #21)"} R[Net#c] == 0;
+  assert {:msg "  Sub-actor action at 3.3 might not preserve the channel invariant (generated #22)"} 0 <= R[Net#d];
+  assert {:msg "  Sub-actor action at 3.3 might not preserve the channel invariant (generated #23)"} 0 <= C[Net#d];
+  assert {:msg "  Sub-actor action at 3.3 might not preserve the channel invariant (generated #24)"} R[Net#d] == 0;
+  assert {:msg "  Sub-actor action at 3.3 might not preserve the channel invariant (generated #25)"} (M[Net#a][0] < 0) && (M[Net#a][1] > 0);
+  assert {:msg "  Sub-actor action at 3.3 might not preserve the channel invariant (generated #26)"} R[Net#a] == (R[Net#b] + C[Net#b]);
+  assert {:msg "  Sub-actor action at 3.3 might not preserve the channel invariant (generated #27)"} (forall idx$: int :: 
     (0 <= idx$) && (idx$ < (R[Net#b] + C[Net#b])) ==> (M[Net#b][idx$] == M[Net#a][idx$])
   );
-  assert {:msg "  20.3: Sub-actor action at 3.3 might not preserve the channel invariant"} (M[Net#a][0] < 0) && (M[Net#a][1] > 0);
-  assert {:msg "  21.3: Sub-actor action at 3.3 might not preserve the channel invariant"} (R[Net#d] + C[Net#d]) == AT#Div(R[Net#b] + 1, 2);
-  assert {:msg "  22.3: Sub-actor action at 3.3 might not preserve the channel invariant"} (R[Net#c] + C[Net#c]) == AT#Div(R[Net#b], 2);
-  assert {:msg "  23.3: Sub-actor action at 3.3 might not preserve the channel invariant"} (forall i: int :: 
+  assert {:msg "  20.3: Sub-actor action at 3.3 might not preserve the channel invariant"} (R[Net#d] + C[Net#d]) == AT#Div(R[Net#b] + 1, 2);
+  assert {:msg "  21.3: Sub-actor action at 3.3 might not preserve the channel invariant"} (R[Net#c] + C[Net#c]) == AT#Div(R[Net#b], 2);
+  assert {:msg "  22.3: Sub-actor action at 3.3 might not preserve the channel invariant"} (forall i: int :: 
     (0 <= i) && (i < R[Net#b]) && (AT#Mod(i, 2) == 0) ==> (M[Net#b][i] == M[Net#d][AT#Div(i, 2)])
   );
-  assert {:msg "  24.3: Sub-actor action at 3.3 might not preserve the channel invariant"} (forall i: int :: 
+  assert {:msg "  23.3: Sub-actor action at 3.3 might not preserve the channel invariant"} (forall i: int :: 
     (0 <= i) && (i < R[Net#b]) && (AT#Mod(i, 2) == 1) ==> (M[Net#b][i] == M[Net#c][AT#Div(i, 2)])
   );
 }
@@ -181,11 +181,11 @@ procedure Net#anon$3#Split#anon$1#5()
   assume 0 <= R[Net#d];
   assume 0 <= C[Net#d];
   assume R[Net#d] == 0;
+  assume (M[Net#a][0] < 0) && (M[Net#a][1] > 0);
   assume R[Net#a] == (R[Net#b] + C[Net#b]);
   assume (forall idx$: int :: 
     (0 <= idx$) && (idx$ < (R[Net#b] + C[Net#b])) ==> (M[Net#b][idx$] == M[Net#a][idx$])
   );
-  assume (M[Net#a][0] < 0) && (M[Net#a][1] > 0);
   assume (R[Net#d] + C[Net#d]) == AT#Div(R[Net#b] + 1, 2);
   assume (R[Net#c] + C[Net#c]) == AT#Div(R[Net#b], 2);
   assume (forall i: int :: 
@@ -202,28 +202,28 @@ procedure Net#anon$3#Split#anon$1#5()
   C[Net#b] := C[Net#b] - 1;
   M[Net#c][R[Net#c] + C[Net#c]] := in#i;
   C[Net#c] := C[Net#c] + 1;
-  assert {:msg "  Sub-actor action at 7.3 might not preserve the channel invariant (generated #26)"} 0 <= R[Net#a];
-  assert {:msg "  Sub-actor action at 7.3 might not preserve the channel invariant (generated #27)"} 0 <= C[Net#a];
-  assert {:msg "  Sub-actor action at 7.3 might not preserve the channel invariant (generated #28)"} (R[Net#a] + C[Net#a]) == C#init[Net#a];
-  assert {:msg "  Sub-actor action at 7.3 might not preserve the channel invariant (generated #29)"} 0 <= R[Net#b];
-  assert {:msg "  Sub-actor action at 7.3 might not preserve the channel invariant (generated #30)"} 0 <= C[Net#b];
-  assert {:msg "  Sub-actor action at 7.3 might not preserve the channel invariant (generated #31)"} 0 <= R[Net#c];
-  assert {:msg "  Sub-actor action at 7.3 might not preserve the channel invariant (generated #32)"} 0 <= C[Net#c];
-  assert {:msg "  Sub-actor action at 7.3 might not preserve the channel invariant (generated #33)"} R[Net#c] == 0;
-  assert {:msg "  Sub-actor action at 7.3 might not preserve the channel invariant (generated #34)"} 0 <= R[Net#d];
-  assert {:msg "  Sub-actor action at 7.3 might not preserve the channel invariant (generated #35)"} 0 <= C[Net#d];
-  assert {:msg "  Sub-actor action at 7.3 might not preserve the channel invariant (generated #36)"} R[Net#d] == 0;
-  assert {:msg "  Sub-actor action at 7.3 might not preserve the channel invariant (generated #37)"} R[Net#a] == (R[Net#b] + C[Net#b]);
-  assert {:msg "  Sub-actor action at 7.3 might not preserve the channel invariant (generated #38)"} (forall idx$: int :: 
+  assert {:msg "  Sub-actor action at 7.3 might not preserve the channel invariant (generated #28)"} 0 <= R[Net#a];
+  assert {:msg "  Sub-actor action at 7.3 might not preserve the channel invariant (generated #29)"} 0 <= C[Net#a];
+  assert {:msg "  Sub-actor action at 7.3 might not preserve the channel invariant (generated #30)"} (R[Net#a] + C[Net#a]) == C#init[Net#a];
+  assert {:msg "  Sub-actor action at 7.3 might not preserve the channel invariant (generated #31)"} 0 <= R[Net#b];
+  assert {:msg "  Sub-actor action at 7.3 might not preserve the channel invariant (generated #32)"} 0 <= C[Net#b];
+  assert {:msg "  Sub-actor action at 7.3 might not preserve the channel invariant (generated #33)"} 0 <= R[Net#c];
+  assert {:msg "  Sub-actor action at 7.3 might not preserve the channel invariant (generated #34)"} 0 <= C[Net#c];
+  assert {:msg "  Sub-actor action at 7.3 might not preserve the channel invariant (generated #35)"} R[Net#c] == 0;
+  assert {:msg "  Sub-actor action at 7.3 might not preserve the channel invariant (generated #36)"} 0 <= R[Net#d];
+  assert {:msg "  Sub-actor action at 7.3 might not preserve the channel invariant (generated #37)"} 0 <= C[Net#d];
+  assert {:msg "  Sub-actor action at 7.3 might not preserve the channel invariant (generated #38)"} R[Net#d] == 0;
+  assert {:msg "  Sub-actor action at 7.3 might not preserve the channel invariant (generated #39)"} (M[Net#a][0] < 0) && (M[Net#a][1] > 0);
+  assert {:msg "  Sub-actor action at 7.3 might not preserve the channel invariant (generated #40)"} R[Net#a] == (R[Net#b] + C[Net#b]);
+  assert {:msg "  Sub-actor action at 7.3 might not preserve the channel invariant (generated #41)"} (forall idx$: int :: 
     (0 <= idx$) && (idx$ < (R[Net#b] + C[Net#b])) ==> (M[Net#b][idx$] == M[Net#a][idx$])
   );
-  assert {:msg "  20.3: Sub-actor action at 7.3 might not preserve the channel invariant"} (M[Net#a][0] < 0) && (M[Net#a][1] > 0);
-  assert {:msg "  21.3: Sub-actor action at 7.3 might not preserve the channel invariant"} (R[Net#d] + C[Net#d]) == AT#Div(R[Net#b] + 1, 2);
-  assert {:msg "  22.3: Sub-actor action at 7.3 might not preserve the channel invariant"} (R[Net#c] + C[Net#c]) == AT#Div(R[Net#b], 2);
-  assert {:msg "  23.3: Sub-actor action at 7.3 might not preserve the channel invariant"} (forall i: int :: 
+  assert {:msg "  20.3: Sub-actor action at 7.3 might not preserve the channel invariant"} (R[Net#d] + C[Net#d]) == AT#Div(R[Net#b] + 1, 2);
+  assert {:msg "  21.3: Sub-actor action at 7.3 might not preserve the channel invariant"} (R[Net#c] + C[Net#c]) == AT#Div(R[Net#b], 2);
+  assert {:msg "  22.3: Sub-actor action at 7.3 might not preserve the channel invariant"} (forall i: int :: 
     (0 <= i) && (i < R[Net#b]) && (AT#Mod(i, 2) == 0) ==> (M[Net#b][i] == M[Net#d][AT#Div(i, 2)])
   );
-  assert {:msg "  24.3: Sub-actor action at 7.3 might not preserve the channel invariant"} (forall i: int :: 
+  assert {:msg "  23.3: Sub-actor action at 7.3 might not preserve the channel invariant"} (forall i: int :: 
     (0 <= i) && (i < R[Net#b]) && (AT#Mod(i, 2) == 1) ==> (M[Net#b][i] == M[Net#c][AT#Div(i, 2)])
   );
 }
@@ -247,11 +247,11 @@ procedure Net#anon$3#Split#anon$2#6()
   assume 0 <= R[Net#d];
   assume 0 <= C[Net#d];
   assume R[Net#d] == 0;
+  assume (M[Net#a][0] < 0) && (M[Net#a][1] > 0);
   assume R[Net#a] == (R[Net#b] + C[Net#b]);
   assume (forall idx$: int :: 
     (0 <= idx$) && (idx$ < (R[Net#b] + C[Net#b])) ==> (M[Net#b][idx$] == M[Net#a][idx$])
   );
-  assume (M[Net#a][0] < 0) && (M[Net#a][1] > 0);
   assume (R[Net#d] + C[Net#d]) == AT#Div(R[Net#b] + 1, 2);
   assume (R[Net#c] + C[Net#c]) == AT#Div(R[Net#b], 2);
   assume (forall i: int :: 
@@ -268,28 +268,28 @@ procedure Net#anon$3#Split#anon$2#6()
   C[Net#b] := C[Net#b] - 1;
   M[Net#d][R[Net#d] + C[Net#d]] := in#i;
   C[Net#d] := C[Net#d] + 1;
-  assert {:msg "  Sub-actor action at 10.3 might not preserve the channel invariant (generated #39)"} 0 <= R[Net#a];
-  assert {:msg "  Sub-actor action at 10.3 might not preserve the channel invariant (generated #40)"} 0 <= C[Net#a];
-  assert {:msg "  Sub-actor action at 10.3 might not preserve the channel invariant (generated #41)"} (R[Net#a] + C[Net#a]) == C#init[Net#a];
-  assert {:msg "  Sub-actor action at 10.3 might not preserve the channel invariant (generated #42)"} 0 <= R[Net#b];
-  assert {:msg "  Sub-actor action at 10.3 might not preserve the channel invariant (generated #43)"} 0 <= C[Net#b];
-  assert {:msg "  Sub-actor action at 10.3 might not preserve the channel invariant (generated #44)"} 0 <= R[Net#c];
-  assert {:msg "  Sub-actor action at 10.3 might not preserve the channel invariant (generated #45)"} 0 <= C[Net#c];
-  assert {:msg "  Sub-actor action at 10.3 might not preserve the channel invariant (generated #46)"} R[Net#c] == 0;
-  assert {:msg "  Sub-actor action at 10.3 might not preserve the channel invariant (generated #47)"} 0 <= R[Net#d];
-  assert {:msg "  Sub-actor action at 10.3 might not preserve the channel invariant (generated #48)"} 0 <= C[Net#d];
-  assert {:msg "  Sub-actor action at 10.3 might not preserve the channel invariant (generated #49)"} R[Net#d] == 0;
-  assert {:msg "  Sub-actor action at 10.3 might not preserve the channel invariant (generated #50)"} R[Net#a] == (R[Net#b] + C[Net#b]);
-  assert {:msg "  Sub-actor action at 10.3 might not preserve the channel invariant (generated #51)"} (forall idx$: int :: 
+  assert {:msg "  Sub-actor action at 10.3 might not preserve the channel invariant (generated #42)"} 0 <= R[Net#a];
+  assert {:msg "  Sub-actor action at 10.3 might not preserve the channel invariant (generated #43)"} 0 <= C[Net#a];
+  assert {:msg "  Sub-actor action at 10.3 might not preserve the channel invariant (generated #44)"} (R[Net#a] + C[Net#a]) == C#init[Net#a];
+  assert {:msg "  Sub-actor action at 10.3 might not preserve the channel invariant (generated #45)"} 0 <= R[Net#b];
+  assert {:msg "  Sub-actor action at 10.3 might not preserve the channel invariant (generated #46)"} 0 <= C[Net#b];
+  assert {:msg "  Sub-actor action at 10.3 might not preserve the channel invariant (generated #47)"} 0 <= R[Net#c];
+  assert {:msg "  Sub-actor action at 10.3 might not preserve the channel invariant (generated #48)"} 0 <= C[Net#c];
+  assert {:msg "  Sub-actor action at 10.3 might not preserve the channel invariant (generated #49)"} R[Net#c] == 0;
+  assert {:msg "  Sub-actor action at 10.3 might not preserve the channel invariant (generated #50)"} 0 <= R[Net#d];
+  assert {:msg "  Sub-actor action at 10.3 might not preserve the channel invariant (generated #51)"} 0 <= C[Net#d];
+  assert {:msg "  Sub-actor action at 10.3 might not preserve the channel invariant (generated #52)"} R[Net#d] == 0;
+  assert {:msg "  Sub-actor action at 10.3 might not preserve the channel invariant (generated #53)"} (M[Net#a][0] < 0) && (M[Net#a][1] > 0);
+  assert {:msg "  Sub-actor action at 10.3 might not preserve the channel invariant (generated #54)"} R[Net#a] == (R[Net#b] + C[Net#b]);
+  assert {:msg "  Sub-actor action at 10.3 might not preserve the channel invariant (generated #55)"} (forall idx$: int :: 
     (0 <= idx$) && (idx$ < (R[Net#b] + C[Net#b])) ==> (M[Net#b][idx$] == M[Net#a][idx$])
   );
-  assert {:msg "  20.3: Sub-actor action at 10.3 might not preserve the channel invariant"} (M[Net#a][0] < 0) && (M[Net#a][1] > 0);
-  assert {:msg "  21.3: Sub-actor action at 10.3 might not preserve the channel invariant"} (R[Net#d] + C[Net#d]) == AT#Div(R[Net#b] + 1, 2);
-  assert {:msg "  22.3: Sub-actor action at 10.3 might not preserve the channel invariant"} (R[Net#c] + C[Net#c]) == AT#Div(R[Net#b], 2);
-  assert {:msg "  23.3: Sub-actor action at 10.3 might not preserve the channel invariant"} (forall i: int :: 
+  assert {:msg "  20.3: Sub-actor action at 10.3 might not preserve the channel invariant"} (R[Net#d] + C[Net#d]) == AT#Div(R[Net#b] + 1, 2);
+  assert {:msg "  21.3: Sub-actor action at 10.3 might not preserve the channel invariant"} (R[Net#c] + C[Net#c]) == AT#Div(R[Net#b], 2);
+  assert {:msg "  22.3: Sub-actor action at 10.3 might not preserve the channel invariant"} (forall i: int :: 
     (0 <= i) && (i < R[Net#b]) && (AT#Mod(i, 2) == 0) ==> (M[Net#b][i] == M[Net#d][AT#Div(i, 2)])
   );
-  assert {:msg "  24.3: Sub-actor action at 10.3 might not preserve the channel invariant"} (forall i: int :: 
+  assert {:msg "  23.3: Sub-actor action at 10.3 might not preserve the channel invariant"} (forall i: int :: 
     (0 <= i) && (i < R[Net#b]) && (AT#Mod(i, 2) == 1) ==> (M[Net#b][i] == M[Net#c][AT#Div(i, 2)])
   );
 }
@@ -313,11 +313,11 @@ procedure Net#anon$3#exit#7()
   assume 0 <= R[Net#d];
   assume 0 <= C[Net#d];
   assume R[Net#d] == 0;
+  assume (M[Net#a][0] < 0) && (M[Net#a][1] > 0);
   assume R[Net#a] == (R[Net#b] + C[Net#b]);
   assume (forall idx$: int :: 
     (0 <= idx$) && (idx$ < (R[Net#b] + C[Net#b])) ==> (M[Net#b][idx$] == M[Net#a][idx$])
   );
-  assume (M[Net#a][0] < 0) && (M[Net#a][1] > 0);
   assume (R[Net#d] + C[Net#d]) == AT#Div(R[Net#b] + 1, 2);
   assume (R[Net#c] + C[Net#c]) == AT#Div(R[Net#b], 2);
   assume (forall i: int :: 
